theories/Operational/Common/OSHandoffContract.v
@@ -1,0 +1,275 @@
+From Stdlib Require Import List Arith Arith.PeanoNat Lia.
+Import ListNotations.
+From RocqSched Require Import Foundation.Base.
+From RocqSched Require Import Multicore.Common.MultiCoreBase.
+From RocqSched Require Import Multicore.Common.Admissibility.
+From RocqSched Require Import Operational.Common.State.
+From RocqSched Require Import Operational.Common.Step.
+From RocqSched Require Import Operational.Common.Invariants.
+From RocqSched Require Import Operational.Common.OSProjectionInterface.
+From RocqSched Require Import Operational.Common.ConcreteExecution.
+From RocqSched Require Import Operational.Common.OSLocalAdapterContract.
+
+Definition ev_consumes_need_resched_on (c : CPU) (ev : OpEvent) : Prop :=
+  match ev with
+  | EvDispatch c' _ => c' = c
+  | EvPreempt c' _ _ => c' = c
+  | _ => False
+  end.
+
+Definition ev_consumes_dispatch_target_on (c : CPU) (j : JobId) (ev : OpEvent) : Prop :=
+  match ev with
+  | EvDispatch c' j' => c' = c /\ j' = j
+  | EvPreempt c' _ j' => c' = c /\ j' = j
+  | EvBlock j' => j' = j
+  | EvComplete j' => j' = j
+  | _ => False
+  end.
+
+Record labeled_concrete_scheduler_handoff_contract
+    {CState : Type}
+    {P : OSLabeledProjection CState}
+    (m : nat)
+    (ex : labeled_concrete_execution P m) : Prop :=
+  mkLabeledConcreteSchedulerHandoffContract {
+    lchc_need_resched_preserved :
+      forall t c,
+        c < m ->
+        op_need_resched
+          (os_to_op_state (osl_to_os_projection P) (lce_trace ex t))
+          c = true ->
+        ~ ev_consumes_need_resched_on
+            c
+            (os_step_label P (lce_trace ex t) (lce_trace ex (S t))) ->
+        op_need_resched
+          (os_to_op_state (osl_to_os_projection P) (lce_trace ex (S t)))
+          c = true;
+    lchc_need_resched_cleared_by_dispatch :
+      forall t c j,
+        c < m ->
+        os_step_label P (lce_trace ex t) (lce_trace ex (S t)) = EvDispatch c j ->
+        op_need_resched
+          (os_to_op_state (osl_to_os_projection P) (lce_trace ex (S t)))
+          c = false;
+    lchc_need_resched_cleared_by_preempt :
+      forall t c old new,
+        c < m ->
+        os_step_label P (lce_trace ex t) (lce_trace ex (S t)) =
+        EvPreempt c old new ->
+        op_need_resched
+          (os_to_op_state (osl_to_os_projection P) (lce_trace ex (S t)))
+          c = false;
+    lchc_dispatch_target_preserved :
+      forall t c j,
+        c < m ->
+        op_dispatch_target
+          (os_to_op_state (osl_to_os_projection P) (lce_trace ex t))
+          c = Some j ->
+        ~ ev_consumes_dispatch_target_on
+            c
+            j
+            (os_step_label P (lce_trace ex t) (lce_trace ex (S t))) ->
+        op_dispatch_target
+          (os_to_op_state (osl_to_os_projection P) (lce_trace ex (S t)))
+          c = Some j;
+    lchc_dispatch_target_consumed_by_dispatch :
+      forall t c j,
+        c < m ->
+        os_step_label P (lce_trace ex t) (lce_trace ex (S t)) = EvDispatch c j ->
+        op_dispatch_target
+          (os_to_op_state (osl_to_os_projection P) (lce_trace ex (S t)))
+          c = None;
+    lchc_dispatch_target_consumed_by_preempt :
+      forall t c old new,
+        c < m ->
+        os_step_label P (lce_trace ex t) (lce_trace ex (S t)) =
+        EvPreempt c old new ->
+        op_dispatch_target
+          (os_to_op_state (osl_to_os_projection P) (lce_trace ex (S t)))
+          c = None;
+    lchc_dispatch_target_cleared_by_block :
+      forall t c j,
+        c < m ->
+        os_step_label P (lce_trace ex t) (lce_trace ex (S t)) = EvBlock j ->
+        op_dispatch_target
+          (os_to_op_state (osl_to_os_projection P) (lce_trace ex (S t)))
+          c <> Some j;
+    lchc_dispatch_target_cleared_by_complete :
+      forall t c j,
+        c < m ->
+        os_step_label P (lce_trace ex t) (lce_trace ex (S t)) = EvComplete j ->
+        op_dispatch_target
+          (os_to_op_state (osl_to_os_projection P) (lce_trace ex (S t)))
+          c <> Some j;
+  }.
+
+Arguments lchc_need_resched_preserved
+  {CState P m ex} _ _ _ _ _.
+Arguments lchc_need_resched_cleared_by_dispatch
+  {CState P m ex} _ _ _ _ _.
+Arguments lchc_need_resched_cleared_by_preempt
+  {CState P m ex} _ _ _ _ _ _.
+Arguments lchc_dispatch_target_preserved
+  {CState P m ex} _ _ _ _ _ _.
+Arguments lchc_dispatch_target_consumed_by_dispatch
+  {CState P m ex} _ _ _ _ _.
+Arguments lchc_dispatch_target_consumed_by_preempt
+  {CState P m ex} _ _ _ _ _ _.
+Arguments lchc_dispatch_target_cleared_by_block
+  {CState P m ex} _ _ _ _ _.
+Arguments lchc_dispatch_target_cleared_by_complete
+  {CState P m ex} _ _ _ _ _.
+
+Lemma local_labeled_concrete_multicore_projection_sound_to_handoff_contract :
+  forall CState (P : OSLabeledProjection CState) jobs adm m
+         (ex : labeled_concrete_execution P m),
+    local_labeled_concrete_multicore_projection_sound jobs adm m ex ->
+    labeled_concrete_scheduler_handoff_contract m ex.
+Proof.
+  intros CState P jobs adm m ex Hmulti.
+  constructor.
+  - intros t c Hlt Hneed Hnotconsume.
+    pose proof (lce_stepwise ex t) as Hstep.
+    destruct (os_step_label P (lce_trace ex t) (lce_trace ex (S t))) eqn:Hev;
+      inversion Hstep; subst; clear Hstep;
+      simpl in *.
+    + exact Hneed.
+    + destruct (op_current (os_to_op_state (osl_to_os_projection P) (lce_trace ex t)) c) as [j'|] eqn:Hcur;
+        simpl.
+      * destruct (Nat.eqb j' j) eqn:Heq.
+        -- reflexivity.
+        -- exact Hneed.
+      * exact Hneed.
+    + destruct (op_current (os_to_op_state (osl_to_os_projection P) (lce_trace ex t)) c) as [j'|] eqn:Hcur;
+        simpl.
+      * destruct (Nat.eqb j' j) eqn:Heq.
+        -- reflexivity.
+        -- exact Hneed.
+      * exact Hneed.
+    + unfold set_need_resched. simpl.
+      destruct (Nat.eqb_spec c0 c).
+      * subst c0. rewrite Nat.eqb_refl. reflexivity.
+      * destruct (Nat.eqb c c0) eqn:Heq.
+        -- apply Nat.eqb_eq in Heq. exfalso. apply n. symmetry. exact Heq.
+        -- exact Hneed.
+    + unfold set_need_resched. simpl.
+      destruct (Nat.eqb_spec c0 c).
+      * subst c0. rewrite Nat.eqb_refl. reflexivity.
+      * destruct (Nat.eqb c c0) eqn:Heq.
+        -- apply Nat.eqb_eq in Heq. exfalso. apply n. symmetry. exact Heq.
+        -- exact Hneed.
+    + exact Hneed.
+    + unfold dispatch_on_cpu, clear_need_resched, set_need_resched. simpl.
+      destruct (Nat.eqb c c0) eqn:Heq.
+      * apply Nat.eqb_eq in Heq. exfalso. apply Hnotconsume. symmetry. exact Heq.
+      * exact Hneed.
+    + unfold preempt_on_cpu, clear_need_resched, set_need_resched. simpl.
+      destruct (Nat.eqb c c0) eqn:Heq.
+      * apply Nat.eqb_eq in Heq. exfalso. apply Hnotconsume. symmetry. exact Heq.
+      * exact Hneed.
+    + exact Hneed.
+    + exact Hneed.
+  - intros t c j Hlt Hdispatch.
+    pose proof (lce_stepwise ex t) as Hstep.
+    rewrite Hdispatch in Hstep.
+    inversion Hstep; subst; clear Hstep.
+    unfold dispatch_on_cpu, clear_need_resched, set_need_resched. simpl.
+    rewrite Nat.eqb_refl.
+    reflexivity.
+  - intros t c old new Hlt Hpreempt.
+    pose proof (lce_stepwise ex t) as Hstep.
+    rewrite Hpreempt in Hstep.
+    inversion Hstep; subst; clear Hstep.
+    unfold preempt_on_cpu, clear_need_resched, set_need_resched. simpl.
+    rewrite Nat.eqb_refl.
+    reflexivity.
+  - intros t c j Hlt Htarget Hnotconsume.
+    pose proof (lce_stepwise ex t) as Hstep.
+    pose proof (lce_struct_inv ex t) as Hinv.
+    destruct (os_step_label P (lce_trace ex t) (lce_trace ex (S t))) eqn:Hev;
+      inversion Hstep; subst; clear Hstep;
+      simpl in *.
+    + exact Htarget.
+    + exact Htarget.
+    + exact Htarget.
+    + exact Htarget.
+    + exact Htarget.
+    + unfold set_dispatch_target. simpl.
+      destruct (Nat.eqb_spec c0 c).
+      * subst c0.
+        rewrite Htarget in H4.
+        discriminate.
+      * destruct (Nat.eqb c c0) eqn:Heq.
+        -- apply Nat.eqb_eq in Heq. exfalso. apply n. symmetry. exact Heq.
+        -- exact Htarget.
+    + unfold dispatch_on_cpu, clear_dispatch_target, set_dispatch_target. simpl.
+      destruct (Nat.eqb c c0) eqn:Heq; simpl in *.
+      * apply Nat.eqb_eq in Heq. subst c0.
+        match goal with
+        | Hpending :
+            op_dispatch_target
+              (os_to_op_state (osl_to_os_projection P) (lce_trace ex t)) c =
+            Some ?jpending |- _ =>
+            rewrite Htarget in Hpending;
+            inversion Hpending; subst
+        end.
+        exfalso. apply Hnotconsume. split; reflexivity.
+      * exact Htarget.
+    + unfold preempt_on_cpu, clear_dispatch_target, set_dispatch_target. simpl.
+      destruct (Nat.eqb c c0) eqn:Heq; simpl in *.
+      * apply Nat.eqb_eq in Heq. subst c0.
+        match goal with
+        | Hpending :
+            op_dispatch_target
+              (os_to_op_state (osl_to_os_projection P) (lce_trace ex t)) c =
+            Some ?jpending |- _ =>
+            rewrite Htarget in Hpending;
+            inversion Hpending; subst
+        end.
+        exfalso. apply Hnotconsume. split; reflexivity.
+      * exact Htarget.
+    + exact Htarget.
+    + exact Htarget.
+  - intros t c j Hlt Hdispatch.
+    pose proof (lce_stepwise ex t) as Hstep.
+    rewrite Hdispatch in Hstep.
+    inversion Hstep; subst; clear Hstep.
+    unfold dispatch_on_cpu, clear_dispatch_target, set_dispatch_target. simpl.
+    rewrite Nat.eqb_refl.
+    reflexivity.
+  - intros t c old new Hlt Hpreempt.
+    pose proof (lce_stepwise ex t) as Hstep.
+    rewrite Hpreempt in Hstep.
+    inversion Hstep; subst; clear Hstep.
+    unfold preempt_on_cpu, clear_dispatch_target, set_dispatch_target. simpl.
+    rewrite Nat.eqb_refl.
+    reflexivity.
+  - intros t c j Hlt Hblock.
+    exact (llcps_block_clears_dispatch_target (llcmps_projection_sound Hmulti) t c j Hlt Hblock).
+  - intros t c j Hlt Hcomplete.
+    pose proof (lce_stepwise ex t) as Hstep.
+    rewrite Hcomplete in Hstep.
+    inversion Hstep; subst; clear Hstep.
+    pose proof (lce_struct_inv ex t) as Hinv.
+    destruct Hinv as [_ _ Hnotin _ Hdispatch].
+    intros Htarget.
+    pose proof (Hdispatch c j Hlt Htarget) as Hin.
+    match goal with
+    | Hrun :
+        op_job_running
+          (os_to_op_state (osl_to_os_projection P) (lce_trace ex t)) j |- _ =>
+        destruct Hrun as [c_run Hcur];
+        exact ((Hnotin c_run j Hcur) Hin)
+    end.
+Qed.
+
+Definition os_local_scheduler_handoff_contract
+    {CState : Type}
+    {P : OSLabeledProjection CState}
+    {jobs : JobId -> Job}
+    {adm : admissible_cpu}
+    {m : nat}
+    (C : os_local_multicore_adapter_contract P jobs adm m)
+  : labeled_concrete_scheduler_handoff_contract m (olac_execution C) :=
+  local_labeled_concrete_multicore_projection_sound_to_handoff_contract
+    CState P jobs adm m (olac_execution C) (olac_sound C).
